

In this lecture, we prove Wilson's Theorem

Theorem: Let  $p$  be a prime number. Then:

$$(p-1)! \equiv -1 \pmod{p}.$$

Example:  $p=2$   $(2-1)! = 1 \equiv -1 \pmod{2}$

$$p=3 \quad (3-1)! = 2 \equiv -1 \pmod{3}$$

$$p=5 \quad (5-1)! = 24 \equiv -1 \pmod{5}$$

$$p=7 \quad (7-1)! = 720 \equiv -1 \pmod{7}$$

Definition: Let  $p$  be a prime, and let  $a \in \{1, 2, \dots, p-1\}$

We define  $\bar{a}$  (or  $a^*$ ) to be the number

in  $\{1, 2, \dots, p-1\}$  satisfying

$$a \cdot \bar{a} \equiv \bar{a} \cdot a \equiv 1 \pmod{p}.$$

$\bar{a}$  is called the inverse of  $a \pmod{p}$ .

Remark: the choice of  $\bar{a}$  is dependent on the modulus. Therefore, sometimes we write  $\bar{a} \pmod{p}$

Example:  $p=7$        $a=5$

$$5 \cdot 3 = 3 \cdot 5 \equiv 1 \pmod{7} \Rightarrow \bar{a} = 3 \pmod{7}$$

$p=11$        $a=4$

$$3 \cdot 4 = 4 \cdot 3 \equiv 1 \pmod{11} \Rightarrow \bar{a} = 3 \pmod{11}$$

Proposition: For  $a \in \{1, 2, \dots, p-1\}$ ,  $\bar{a}$  always exists and it is unique.

Proof: Existence: (We need to show: for any  $a \in \{1, 2, \dots, p-1\}$  we can  $\bar{a} \in \{1, 2, \dots, p-1\}$ )

Let  $a \in \{1, 2, \dots, p-1\}$ . Then  $\gcd(a, p) = 1$ .

Then we can find  $r, s$  such that

$$ra + sp = 1. \quad \text{This also shows: } \gcd(r, p) = 1.$$

By Euclidean algorithm, we can find  $q$  and  $r_0$  such that

$$r = q \cdot p + r_0 \quad \text{with } 1 \leq r_0 \leq p-1.$$

Substitute this into the previous equation:

$$r_0 a + p(qa + s) = 1$$

This shows:  $ra = ar \equiv 1 \pmod{p}$

Uniqueness: We need to show: if  
 $aa_1 = a_1a \equiv 1 \pmod{p} \quad a_1 \in \{1, \dots, p-1\}$   
and  
 $aa_2 = a_2a \equiv 1 \pmod{p} \quad a_2 \in \{1, \dots, p-1\}$   
then  $a_1 = a_2 \pmod{p}$

Suppose that  $aa_1 \equiv a_1a \equiv 1 \pmod{p} \quad a_1 \in \{1, \dots, p-1\}$   
 $aa_2 \equiv a_2a \equiv 1 \pmod{p} \quad a_2 \in \{1, \dots, p-1\}$

$$\text{Then } a(a_1 - a_2) \equiv 1 - 1 \pmod{p}$$

$$\Rightarrow a(a_1 - a_2) \equiv 0 \pmod{p}$$

$$a \in \{1, \dots, p-1\} \quad \gcd(a, p) = 1$$

The equation becomes:  $a_1 \equiv a_2 \pmod{p}$

$$a_1, a_2 \in \{1, \dots, p-1\} \Rightarrow a_1 = a_2$$

□

Fact: Let  $p$  fixed. Then:

$$(1) \quad \overline{1} = 1$$

$$(2) \quad \overline{p-1} = p-1 \equiv -1 \pmod{p}$$

(3) For  $a \in \{1, 2, \dots, p-1\}$ ,  $\overline{\overline{a}} = a$ .

Proof: (1)  $1 \cdot 1 \equiv 1 \pmod{p} \Rightarrow 1 = \overline{1}$

(2)  $(p-1) \cdot (p-1) = p^2 - 2p + 1 \equiv 1 \pmod{p}$

$\Rightarrow \overline{p-1} = p-1 \quad p-1 \equiv -1 \pmod{p} \quad \checkmark$

(1) By definition:

$$a \overline{a} = \overline{a} a \equiv 1 \pmod{p}$$

Therefore:

$$\overline{a} a = a \overline{a} \equiv 1 \pmod{p}$$

Hence:  $\overline{\overline{a}} = a$ .

□

Proposition: Let  $p$  be a prime, and  $a \in \{1, \dots, p-1\}$ .

Then  $a = \overline{a}$  if and only if  $a = 1$  or  $p-1$ .

In other words,  $a \neq \overline{a}$  for  $a \in \{2, \dots, p-2\}$

Proof: Notice that:  $a = \overline{a}$  if and only if  $a \cdot a \equiv 1 \pmod{p}$   
if and only if  $a$  is a solution  
for  $x^2 \equiv 1 \pmod{p}$ .

$a=1$  and  $a=p-1$  are solutions for  $x^2 \equiv 1 \pmod{p}$ .

Therefore, it suffices to show: the congruent equation:

$$x^2 \equiv 1 \pmod{p}$$

has at most two solutions.

Proof by contradiction: suppose not, we have:

$$a_1^2 \equiv a_2^2 \equiv a_3^2 \equiv 1 \pmod{p} \text{ for } a_1, a_2, a_3 \in \{1, \dots, p-1\}$$

and they are distinct numbers

$$\text{This implies: } a_1^2 \equiv a_2^2 \pmod{p} \Rightarrow p \mid a_1^2 - a_2^2 = (a_1 - a_2)(a_1 + a_2)$$

$$a_1^2 \equiv a_3^2 \pmod{p} \Rightarrow p \mid a_1^2 - a_3^2 = (a_1 - a_3)(a_1 + a_3)$$

If  $p \mid a_1 - a_2$ , then  $a_1, a_2 \in \{1, \dots, p-1\}$  implies that  $a_1 = a_2$

If  $p \mid a_1 - a_3$ , then  $a_1, a_3 \in \{1, \dots, p-1\}$  implies that  $a_1 = a_3$

$$\text{Then } p \mid a_1 + a_2 \text{ and } p \mid a_1 + a_3$$

$$\Rightarrow p \mid a_2 - a_3$$

This is impossible since  $a_2 \neq a_3 \in \{1, \dots, p-1\}$

A contradiction!

Therefore:  $x^2 \equiv 1 \pmod{p}$  has at most two solutions.  $\square$

Proof of Theorem: Let  $a \in \{2, \dots, p-2\}$

Then by the uniqueness of  $\bar{a}$  and the Fact,

$$\bar{a} \in \{2, \dots, p-2\}$$

Then we write:

$$(p-1)! = 1 \cdot 2 \cdot 3 \cdots (p-3)(p-2)(p-1)$$

We leave the term 1 and the term  $(p-1)$ .

For other terms, we group it with its inverse.

$$\text{Then } 1 \cdot 2 \cdot 3 \cdots (p-3)(p-2)(p-1)$$

$$\equiv 1 \cdot (2 \cdot \bar{2} \cdots ) \cdot (p-1)$$

$$\equiv 1 \cdot (p-1) \equiv p-1.$$

$$\equiv -1 \pmod{p}$$

□